Renaming types to begin with lowercase

src/Circuit.fst
@@ -8,27 +8,27 @@ module Circuit
 open Set
 open Total
 
-type Gate =
+type gate =
   | RCNOT of int * int
   | RTOFF of int * int * int
   | RNOT  of int
 
-type Circuit = list Gate
+type circuit = list gate
 
-val prettyPrintGate    : Gate -> string
-val prettyPrintCircuit : Circuit -> list string
+val prettyPrintGate    : gate -> string
+val prettyPrintCircuit : circuit -> list string
 
-val applyGate          : state -> Gate -> Tot state
-val evalCirc           : Circuit -> state -> Tot state
-val wfGate             : Gate -> Tot bool
-val wfCirc             : Circuit -> Tot bool
-val used               : int -> Circuit -> Tot bool
-val uses               : Circuit -> Tot (set int)
-val modded             : int -> Circuit -> Tot bool
-val mods               : Circuit -> Tot (set int)
-val ctrl               : int -> Circuit -> Tot bool
-val ctrls              : Circuit -> Tot (set int)
-val uncompute          : Circuit -> int -> Tot Circuit
+val applyGate          : state -> gate -> Tot state
+val evalCirc           : circuit -> state -> Tot state
+val wfGate             : gate -> Tot bool
+val wfCirc             : circuit -> Tot bool
+val used               : int -> circuit -> Tot bool
+val uses               : circuit -> Tot (set int)
+val modded             : int -> circuit -> Tot bool
+val mods               : circuit -> Tot (set int)
+val ctrl               : int -> circuit -> Tot bool
+val ctrls              : circuit -> Tot (set int)
+val uncompute          : circuit -> int -> Tot circuit
 
 (* Printing *)
 let prettyPrintGate gate = match gate with
@@ -94,25 +94,25 @@ let rec uncompute circ targ = match circ with
 (** Verification utilities *)
 
 (* Lemmas about modified bits *)
-val ref_imp_use : gates:Circuit ->
+val ref_imp_use : gates:circuit ->
   Lemma (forall i. modded i gates \/ ctrl i gates <==> used i gates)
 let rec ref_imp_use gates = match gates with
   | [] -> ()
   | x::xs -> ref_imp_use xs
 
-val mods_sub_uses : gates:Circuit ->
+val mods_sub_uses : gates:circuit ->
   Lemma (subset (mods gates) (uses gates))
 let mods_sub_uses gates = ref_imp_use gates
 
-val ctrls_sub_uses : gates:Circuit ->
+val ctrls_sub_uses : gates:circuit ->
   Lemma (subset (ctrls gates) (uses gates))
 let ctrls_sub_uses gates = ref_imp_use gates
 
-val apply_mod : st:state -> x:Gate ->
+val apply_mod : st:state -> x:gate ->
   Lemma (agree_on st (applyGate st x) (complement (mods [x])))
 let apply_mod st x = ()
 
-val eval_mod : st:state -> gates:Circuit ->
+val eval_mod : st:state -> gates:circuit ->
   Lemma (agree_on st (evalCirc gates st) (complement (mods gates))) (decreases gates)
 let rec eval_mod st gates = match gates with
   | [] -> ()
@@ -120,7 +120,7 @@ let rec eval_mod st gates = match gates with
 
 (* Append lemmas, uses SMTPat to expand out automatically *)
 
-val evalCirc_append : l1:Circuit -> l2:Circuit -> st:state ->
+val evalCirc_append : l1:circuit -> l2:circuit -> st:state ->
   Lemma (requires true)
         (ensures (evalCirc (l1@l2) st = evalCirc l2 (evalCirc l1 st)))
   [SMTPat (evalCirc (l1@l2) st)]
@@ -128,7 +128,7 @@ let rec evalCirc_append l1 l2 st = match l1 with
   | [] -> ()
   | x::xs -> evalCirc_append xs l2 (applyGate st x)
 
-val use_append : i:int -> x:Circuit -> y:Circuit ->
+val use_append : i:int -> x:circuit -> y:circuit ->
   Lemma (requires true)
         (ensures  (used i (x@y) <==> used i x \/ used i y))
   [SMTPat (used i (x@y))]
@@ -136,14 +136,14 @@ let rec use_append i x y = match x with
   | [] -> ()
   | x::xs -> use_append i xs y
 
-val uses_append : x:Circuit -> y:Circuit ->
+val uses_append : x:circuit -> y:circuit ->
   Lemma (requires true)
         (ensures  (uses (x@y) = union (uses x) (uses y)))
   [SMTPat (uses (x@y))]
 let rec uses_append x y =
   lemma_equal_intro (uses (x@y)) (union (uses x) (uses y))
 
-val mod_append : i:int -> l1:Circuit -> l2:Circuit ->
+val mod_append : i:int -> l1:circuit -> l2:circuit ->
   Lemma (requires true)
         (ensures  (modded i (l1@l2) <==> modded i l1 \/ modded i l2))
   [SMTPat (modded i (l1@l2))]
@@ -151,14 +151,14 @@ let rec mod_append i l1 l2 = match l1 with
   | [] -> ()
   | x::xs -> mod_append i xs l2
 
-val mods_append : x:Circuit -> y:Circuit ->
+val mods_append : x:circuit -> y:circuit ->
   Lemma (requires true)
         (ensures  (mods (x@y) = union (mods x) (mods y)))
   [SMTPat (mods (x@y))]
 let rec mods_append x y =
   lemma_equal_intro (mods (x@y)) (union (mods x) (mods y))
 
-val ctrl_append : i:int -> x:Circuit -> y:Circuit ->
+val ctrl_append : i:int -> x:circuit -> y:circuit ->
   Lemma (requires true)
         (ensures  (ctrl i (x@y) <==> ctrl i x \/ ctrl i y))
   [SMTPat (ctrl i (x@y))]
@@ -166,14 +166,14 @@ let rec ctrl_append i x y = match x with
   | [] -> ()
   | x::xs -> ctrl_append i xs y
 
-val ctrls_append : x:Circuit -> y:Circuit ->
+val ctrls_append : x:circuit -> y:circuit ->
   Lemma (requires true)
         (ensures  (ctrls (x@y) = union (ctrls x) (ctrls y)))
   [SMTPat (ctrls (x@y))]
 let rec ctrls_append x y =
   lemma_equal_intro (ctrls (x@y)) (union (ctrls x) (ctrls y))
 
-val wf_append : x:Circuit -> y:Circuit ->
+val wf_append : x:circuit -> y:circuit ->
   Lemma (requires (wfCirc x /\ wfCirc y))
         (ensures  (wfCirc (x@y)))
   [SMTPat (wfCirc (x@y))]
@@ -182,7 +182,7 @@ let rec wf_append x y = match x with
   | x::xs -> wf_append xs y
 
 (* Lemmas about reversibility *)
-val rev_uses : circ:Circuit ->
+val rev_uses : circ:circuit ->
   Lemma (requires true)
         (ensures (uses circ = uses (List.rev circ)))
   [SMTPat (uses (List.rev circ))]
@@ -193,7 +193,7 @@ let rec rev_uses circ = match circ with
     rev_uses xs;
     lemma_equal_intro (uses circ) (uses (List.rev circ))
 
-val rev_mods : circ:Circuit ->
+val rev_mods : circ:circuit ->
   Lemma (requires true)
         (ensures (mods circ = mods (List.rev circ)))
   [SMTPat (mods (List.rev circ))]
@@ -204,7 +204,7 @@ let rec rev_mods circ = match circ with
     rev_mods xs;
     lemma_equal_intro (mods circ) (mods (List.rev circ))
 
-val rev_ctrls : circ:Circuit ->
+val rev_ctrls : circ:circuit ->
   Lemma (requires true)
         (ensures (ctrls circ = ctrls (List.rev circ)))
   [SMTPat (ctrls (List.rev circ))]
@@ -215,16 +215,16 @@ let rec rev_ctrls circ = match circ with
     rev_ctrls xs;
     lemma_equal_intro (ctrls circ) (ctrls (List.rev circ))
 
-val evalCirc_append_rev : x:Circuit -> y:Circuit -> st:state ->
+val evalCirc_append_rev : x:circuit -> y:circuit -> st:state ->
   Lemma (evalCirc (List.rev (x@y)) st = evalCirc (List.rev x) (evalCirc (List.rev y) st))
 let evalCirc_append_rev x y st = ListProperties.rev_append x y
 
-val rev_gate : gate:Gate -> st:state ->
+val rev_gate : gate:gate -> st:state ->
   Lemma (requires (wfGate gate))
         (ensures  (Equal (applyGate (applyGate st gate) gate) st))
 let rev_gate gate st = lemma_map_equal_intro (applyGate (applyGate st gate) gate) st
 
-val rev_inverse : circ:Circuit -> st:state ->
+val rev_inverse : circ:circuit -> st:state ->
   Lemma (requires (wfCirc circ))
         (ensures  (Equal (evalCirc (circ@(List.rev circ)) st) st))
 let rec rev_inverse circ st = match circ with
@@ -235,12 +235,12 @@ let rec rev_inverse circ st = match circ with
     rev_gate x st;
     lemma_map_equal_intro (evalCirc (circ@(List.rev circ)) st) st
 
-val applyGate_state_swap : x:Gate -> st:state -> st':state -> dom:set int ->
+val applyGate_state_swap : x:gate -> st:state -> st':state -> dom:set int ->
   Lemma (requires (subset (ctrls [x]) dom /\ agree_on st st' dom))
         (ensures  (agree_on (applyGate st x) (applyGate st' x) dom))
 let applyGate_state_swap x st st' dom = ()
 
-val evalCirc_state_swap : circ:Circuit -> st:state -> st':state -> dom:set int ->
+val evalCirc_state_swap : circ:circuit -> st:state -> st':state -> dom:set int ->
   Lemma (requires (subset (ctrls circ) dom /\ agree_on st st' dom))
         (ensures  (agree_on (evalCirc circ st) (evalCirc circ st') dom))
 let rec evalCirc_state_swap circ st st' dom = match circ with
@@ -250,7 +250,7 @@ let rec evalCirc_state_swap circ st st' dom = match circ with
     evalCirc_state_swap xs (applyGate st x) (applyGate st' x) dom
 
 (* Lemmas for uncomputing after copying to a target *)
-val bennett : comp:Circuit -> copy:Circuit -> st:state ->
+val bennett : comp:circuit -> copy:circuit -> st:state ->
   Lemma (requires (wfCirc comp /\ disjoint (uses comp) (mods copy)))
         (ensures  (agree_on st (evalCirc (comp@copy@(List.rev comp)) st) (uses comp)))
 let bennett comp copy st =
@@ -261,13 +261,13 @@ let bennett comp copy st =
     evalCirc_state_swap (List.rev comp) st' st'' (uses comp);
     rev_inverse comp st
 
-val uncompute_targ : circ:Circuit -> targ:int ->
+val uncompute_targ : circ:circuit -> targ:int ->
   Lemma (not (modded targ (uncompute circ targ)))
 let rec uncompute_targ circ targ = match circ with
   | [] -> ()
   | x::xs -> uncompute_targ xs targ
 
-val uncompute_wf : circ:Circuit -> targ:int ->
+val uncompute_wf : circ:circuit -> targ:int ->
   Lemma (requires (wfCirc circ))
         (ensures  (wfCirc (uncompute circ targ)))
   [SMTPat (wfCirc (uncompute circ targ))]
@@ -275,21 +275,21 @@ let rec uncompute_wf circ targ = match circ with
   | [] -> ()
   | x::xs -> uncompute_wf xs targ
 
-val uncompute_uses_subset : circ:Circuit -> targ:int ->
+val uncompute_uses_subset : circ:circuit -> targ:int ->
   Lemma (requires (wfCirc circ))
         (ensures  (subset (uses (uncompute circ targ)) (uses circ)))
 let rec uncompute_uses_subset circ targ = match circ with
   | [] -> ()
   | x::xs -> uncompute_uses_subset xs targ
 
-val uncompute_ctrls_subset : circ:Circuit -> targ:int ->
+val uncompute_ctrls_subset : circ:circuit -> targ:int ->
   Lemma (requires (wfCirc circ))
         (ensures  (subset (ctrls (uncompute circ targ)) (ctrls circ)))
 let rec uncompute_ctrls_subset circ targ = match circ with
   | [] -> ()
   | x::xs -> uncompute_ctrls_subset xs targ
 
-val uncompute_agree : circ:Circuit -> targ:int -> st:state ->
+val uncompute_agree : circ:circuit -> targ:int -> st:state ->
   Lemma (requires (wfCirc circ /\ not (ctrl targ circ)))
         (ensures  (agree_on (evalCirc circ st)
                             (evalCirc (uncompute circ targ) st)
@@ -308,7 +308,7 @@ let rec uncompute_agree circ targ st = match circ with
     else uncompute_agree xs targ (applyGate st x)
 
 
-val uncompute_mixed_inverse : circ:Circuit -> targ:int -> st:state ->
+val uncompute_mixed_inverse : circ:circuit -> targ:int -> st:state ->
   Lemma (requires (wfCirc circ /\ not (ctrl targ circ)))
         (ensures  (agree_on st (evalCirc (List.rev (uncompute circ targ))
                                          (evalCirc circ st))
